Splitting geometric logic boilerplate inside its own file.

coquand_geometrical_logic/dynamic.v
@@ -1,4 +1,4 @@
-Require Import seq syntax deduction.
+Require Import seq syntax deduction geometric.
 
 Set Primitive Projections.
 
@@ -13,60 +13,7 @@ Notation atom := Sig.(sig_atom).
 Notation atom_arity := Sig.(sig_atom_arity).
 Notation term := (@term Sig).
 Notation form := (@form Sig).
-
-Definition atomic Σ := { a : atom & seq (term Σ) (atom_arity a) }.
-
-Definition subst_atomic {Σ Σ' : nat} (σ : seq (term Σ') Σ) (a : atomic Σ) : atomic Σ' :=
-match a with
-| existT _ α args => existT _ α (args >> σ)
-end.
-
-Definition nlift_atomic {Σ} Σ' (a : atomic Σ) : atomic (Σ' + Σ) :=
-  subst_atomic (init (funcomp var_term (shift_p Σ'))) a.
-
-Definition mAtm {Σ} (a : atomic Σ) : form Σ :=
-match a with existT _ α args => Atm α args end.
-
-Fixpoint nAll (Σ : nat) (A : form Σ) : form 0 :=
-match Σ return form Σ -> form 0 with
-| 0 => fun A => A
-| S Σ => fun A => nAll Σ (All A)
-end A.
-
-Fixpoint nCnj {Σ : nat} (Φ : list (atomic Σ)) : form Σ := match Φ with
-| nil => Top
-| cons A Φ => Cnj (mAtm A) (nCnj Φ)
-end.
-
-Fixpoint nExs {Σ Σ' : nat} (A : form (Σ' + Σ)) : form Σ :=
-match Σ' return form (Σ' + Σ) -> form Σ with
-| 0 => fun A => A
-| S Σ' => fun A => nExs (Exs A)
-end A.
-
-Fixpoint nSplit {Σ : nat} (Ψ : list {Σ' : nat & list (atomic (Σ' + Σ))}) : form Σ := match Ψ with
-| nil => Bot
-| cons (existT _ Σ' Φ) Ψ => Dsj (nExs (nCnj Φ)) (nSplit Ψ)
-end.
-
-Record geometric := {
-  geom_ctx : nat;
-  geom_hyp : list (atomic geom_ctx);
-  geom_ccl : list {Σ : nat & list (atomic (Σ + geom_ctx))};
-}.
-
-Definition of_geometric (G : geometric) : form 0 :=
-  nAll G.(geom_ctx) (Arr (nCnj G.(geom_hyp)) (nSplit G.(geom_ccl))).
-
-Record GTheory := {
-  gthy_idx : Type;
-  gthy_axm : forall (i : gthy_idx), geometric;
-}.
-
-Definition of_gtheory (T : GTheory) : Theory := {|
-  thy_idx := T.(gthy_idx);
-  thy_axm := fun i => of_geometric (T.(gthy_axm) i);
-|}.
+Notation atomic := (@atomic Sig).
 
 Record ℙ := mkℙ {
   idxℙ : nat;
@@ -166,7 +113,7 @@ Definition isMon {Ω} (A : forall Ω', Ω' ≤ Ω -> Type) :=
 
 Section Interp.
 
-Variable T : GTheory.
+Variable T : @GTheory Sig.
 
 Inductive Forall {A : Type} (P : A -> Type) : list A -> Type :=
 | Forall_nil : Forall P nil
@@ -646,7 +593,7 @@ Defined.
 
 Lemma interp_nSplit : forall Σ Ψ Ω (ρ : seq (term Ω.(idxℙ)) Σ) (o : fin (length Ψ)),
   match nth Ψ o with existT _ Σ' Φ => { σ : _ & @interp _ (nCnj Φ) Ω (scons_p σ ρ) } end ->
-  interp (@nSplit Σ Ψ) ρ.
+  interp (@nSplit _ Σ Ψ) ρ.
 Proof.
 induction Ψ as [|[Σ' Φ] Ψ IHΨ]; intros Ω ρ o p; cbn in *.
 + destruct o.
@@ -748,7 +695,7 @@ unshelve refine (ask _ _ i (lift_le σ (γ ∘ β)) _ _); fold φ.
 Qed.
 
 Lemma interp_sound : forall Σ Γ (A : form Σ) Ω (ρ : seq (term Ω.(idxℙ)) Σ),
-  proof (of_gtheory T) Σ Γ A -> Forall (fun X => interp X ρ) Γ -> interp A ρ.
+  proof T Σ Γ A -> Forall (fun X => interp X ρ) Γ -> interp A ρ.
 Proof.
 intros Σ Γ A Ω ρ π; revert Ω ρ; induction π; intros Ω ρ γ; cbn in *.
 + exfalso; congruence.
