coquand_geometrical_logic/geometric.v
@@ -1,0 +1,72 @@
+Require Import seq syntax deduction.
+
+Set Primitive Projections.
+
+Section geometric.
+
+Context {Sig : sig}.
+
+Notation symb := Sig.(sig_symb).
+Notation symb_arity := Sig.(sig_symb_arity).
+Notation atom := Sig.(sig_atom).
+Notation atom_arity := Sig.(sig_atom_arity).
+Notation term := (@term Sig).
+Notation form := (@form Sig).
+
+Definition atomic Σ := { a : atom & seq (term Σ) (atom_arity a) }.
+
+Definition subst_atomic {Σ Σ' : nat} (σ : seq (term Σ') Σ) (a : atomic Σ) : atomic Σ' :=
+match a with
+| existT _ α args => existT _ α (args >> σ)
+end.
+
+Definition nlift_atomic {Σ} Σ' (a : atomic Σ) : atomic (Σ' + Σ) :=
+  subst_atomic (init (funcomp var_term (shift_p Σ'))) a.
+
+Definition mAtm {Σ} (a : atomic Σ) : form Σ :=
+match a with existT _ α args => Atm α args end.
+
+Fixpoint nAll (Σ : nat) (A : form Σ) : form 0 :=
+match Σ return form Σ -> form 0 with
+| 0 => fun A => A
+| S Σ => fun A => nAll Σ (All A)
+end A.
+
+Fixpoint nCnj {Σ : nat} (Φ : list (atomic Σ)) : form Σ := match Φ with
+| nil => Top
+| cons A Φ => Cnj (mAtm A) (nCnj Φ)
+end.
+
+Fixpoint nExs {Σ Σ' : nat} (A : form (Σ' + Σ)) : form Σ :=
+match Σ' return form (Σ' + Σ) -> form Σ with
+| 0 => fun A => A
+| S Σ' => fun A => nExs (Exs A)
+end A.
+
+Fixpoint nSplit {Σ : nat} (Ψ : list {Σ' : nat & list (atomic (Σ' + Σ))}) : form Σ := match Ψ with
+| nil => Bot
+| cons (existT _ Σ' Φ) Ψ => Dsj (nExs (nCnj Φ)) (nSplit Ψ)
+end.
+
+Record geometric := {
+  geom_ctx : nat;
+  geom_hyp : list (atomic geom_ctx);
+  geom_ccl : list {Σ : nat & list (atomic (Σ + geom_ctx))};
+}.
+
+Definition of_geometric (G : geometric) : form 0 :=
+  nAll G.(geom_ctx) (Arr (nCnj G.(geom_hyp)) (nSplit G.(geom_ccl))).
+
+Record GTheory := {
+  gthy_idx : Type;
+  gthy_axm : forall (i : gthy_idx), geometric;
+}.
+
+Definition of_gtheory (T : GTheory) : Theory := {|
+  thy_idx := T.(gthy_idx);
+  thy_axm := fun i => of_geometric (T.(gthy_axm) i);
+|}.
+
+End geometric.
+
+Coercion of_gtheory : GTheory >-> Theory.
